src/arrcp_mcl.lean
@@ -1,14 +1,40 @@
 import mcl
+import parlang
 open mcl
 
 namespace arrcp_mcl
 
 def sig : signature
-| _ := type.int
+| _ := { scope := scope.global, type := type.int }
 
 def arrcp₁ : mclp sig := mclp.intro (λ m, 10) (mclk.global_assign "b" (expression.const_int 7 (by refl)))
 
 def arrcp₂ : mclp sig := mclp.intro (λ m, 10) (mclk.global_assign "c" (expression.const_int 9 (by refl)))
+
+def d {α : Type} {b : α} (a c : α) := a = b ∧ b = c
+
+example (c) : mclp_to_program arrcp₁ = c := begin
+    rw arrcp₁,
+    rw [mclp_to_program, mclk_to_kernel, prepend_load_expr, load_global_vars_for_expr],
+    unfold append,
+    rw list.append,
+    rw parlang.list_to_kernel_seq,
+    repeat {rw list.foldl},
+end
+
+#eval mclp_to_program arrcp₁
+#check ```(mclp_to_program arrcp₁)
+#print mclp_to_program
+
+def X : ℕ → ℕ := λ n, n + 2
+
+meta def num_args : expr → nat
+| (expr.app f a) := num_args f + 1
+| e:=0
+
+#check X
+#check `(X)
+#eval parlang.expr.repr `(X)
 
 example : mclp_rel (λ m₁ m₂, sorry) arrcp₁ arrcp₂ (λ m₁ m₂, sorry) := begin
     
